```ad-question
title:Question
collapse:open
$$
\int \frac{x^2-1}{x^4+1}dx
$$
```

解:
$$\begin{align}
\int \frac{x^2-1}{x^4+1}dx &= \int \frac{1-\frac{1}{x^2}}{\frac{1}{x^2} + x^2}dx \\
&= \int \frac{1-\frac{1}{x^2}}{\frac{1}{x^2} + x^2-2+2}dx \\
&= \int \frac{d(x +\frac{1}{x})}{(x+\frac{1}{x})^2-2} \\
令x+\frac{1}{x} &= t \\
&= \int \frac{dt}{t^2 -2} \\
&= \int \frac{dt}{(t+\sqrt{2})(t-\sqrt{2})} \\
&= \frac{1}{2\sqrt{2}}\int \frac{1}{{{t}-\sqrt{2}}}-\frac{1}{{{t}+\sqrt{2}}}dt \\
&= \int \frac{1}{2\sqrt{2}}|\ln \frac{t-\sqrt{2}}{t+\sqrt{2}}|+c
\end{align}$$

```ad-important
title:Important
collapse:open
$$\begin{align}
(x+\frac{1}{x})' = 1-\frac{1}{x^2} \\
(x-\frac{1}{x})' = 1+\frac{1}{x^2}
\end{align}$$
```

```ad-question
title:Question
collapse:open
$$\begin{align}
\int \frac{x^2+1}{x^4+1}dx
\end{align}$$
```

$$\begin{align}
\int \frac{x^2+1}{x^4+1}dx &= \int \frac{1+\frac{1}{x^2}}{\frac{1}{x^2}+x^2}dx \\
&= \int \frac{1+\frac{1}{x^2}}{\frac{1}{x^2}+x^2-2+2}dx \\
&= \int \frac{d(x-\frac{1}{x})}{(x-\frac{1}{x})^2+2} \\
令 x- \frac{1}{x} = t \\
&= \int \frac{dt}{t^2+2} \\
&= \frac{\sqrt{2}}{2}\int \frac{d\frac{\sqrt{2}}{2}t}{(\frac{\sqrt{2}}{2}t)^2+1} \\
&= \frac{\sqrt{2}}{2} \arctan\frac{\sqrt{2}}{2}t+C \\
t换成x-\frac{1}{x}
\end{align}$$

```ad-question
title:Question
collapse:open
$$
\int \frac{x^2}{1+x^4}dx
$$
```

$$\begin{align}
\int \frac{x^2}{1+x^4}dx &= \frac{1}{2} \int \frac{(x^2+1)+(x^2-1)}{1+x^4}dx \\
&= \frac{1}{2}\int \frac{(x^2+1)}{1+x^4}dx + \frac{1}{2}\int\frac{(x^2-1)}{1+x^4}dx \\
思路同上
\end{align}$$

```ad-question
title:Question
collapse:open
$$
\int \frac{x^4+1}{x^6+1}dx
$$
```

$$\begin{align}
\int \frac{x^4+1}{x^6+1}dx &= \int \frac{(x^4-x^2+1)+x^2}{x^6+1}dx \\
&= \int \frac{(x^4-x^2+1)}{(x^2+1)(x^4-x^2+1)}
dx + \frac{1}{3}\int \frac{dx^3}{x^6+1} \\
&= \arctan x + \frac{1}{3}\arctan x^3 +C
\end{align}$$
